moved "open" operations from Heap.thy to Array.thy and Ref.thy

src/HOL/Imperative_HOL/Array.thy
@@ -8,24 +8,132 @@ theory Array
 imports Heap_Monad
 begin
 
+subsection {* Primitive layer *}
+
+definition 
+  array_present :: "'a\<Colon>heap array \<Rightarrow> heap \<Rightarrow> bool" where
+  "array_present a h \<longleftrightarrow> addr_of_array a < lim h"
+
+definition
+  get_array :: "'a\<Colon>heap array \<Rightarrow> heap \<Rightarrow> 'a list" where
+  "get_array a h = map from_nat (arrays h (TYPEREP('a)) (addr_of_array a))"
+
+definition
+  set_array :: "'a\<Colon>heap array \<Rightarrow> 'a list \<Rightarrow> heap \<Rightarrow> heap" where
+  "set_array a x = 
+  arrays_update (\<lambda>h. h(TYPEREP('a) := ((h(TYPEREP('a))) (addr_of_array a:=map to_nat x))))"
+
+definition array :: "'a list \<Rightarrow> heap \<Rightarrow> 'a\<Colon>heap array \<times> heap" where
+  "array xs h = (let
+     l = lim h;
+     r = Array l;
+     h'' = set_array r xs (h\<lparr>lim := l + 1\<rparr>)
+   in (r, h''))"
+
+definition length :: "'a\<Colon>heap array \<Rightarrow> heap \<Rightarrow> nat" where
+  "length a h = List.length (get_array a h)"
+  
+definition change :: "'a\<Colon>heap array \<Rightarrow> nat \<Rightarrow> 'a \<Rightarrow> heap \<Rightarrow> heap" where
+  "change a i x h = set_array a ((get_array a h)[i:=x]) h"
+
+text {* Properties of imperative arrays *}
+
+text {* FIXME: Does there exist a "canonical" array axiomatisation in
+the literature?  *}
+
+definition noteq_arrs :: "('a\<Colon>heap) array \<Rightarrow> ('b\<Colon>heap) array \<Rightarrow> bool" (infix "=!!=" 70) where
+  "r =!!= s \<longleftrightarrow> TYPEREP('a) \<noteq> TYPEREP('b) \<or> addr_of_array r \<noteq> addr_of_array s"
+
+lemma noteq_arrs_sym: "a =!!= b \<Longrightarrow> b =!!= a"
+  and unequal_arrs [simp]: "a \<noteq> a' \<longleftrightarrow> a =!!= a'"
+  unfolding noteq_arrs_def by auto
+
+lemma noteq_arrs_irrefl: "r =!!= r \<Longrightarrow> False"
+  unfolding noteq_arrs_def by auto
+
+lemma present_new_arr: "array_present a h \<Longrightarrow> a =!!= fst (array xs h)"
+  by (simp add: array_present_def noteq_arrs_def array_def Let_def)
+
+lemma array_get_set_eq [simp]: "get_array r (set_array r x h) = x"
+  by (simp add: get_array_def set_array_def o_def)
+
+lemma array_get_set_neq [simp]: "r =!!= s \<Longrightarrow> get_array r (set_array s x h) = get_array r h"
+  by (simp add: noteq_arrs_def get_array_def set_array_def)
+
+lemma set_array_same [simp]:
+  "set_array r x (set_array r y h) = set_array r x h"
+  by (simp add: set_array_def)
+
+lemma array_set_set_swap:
+  "r =!!= r' \<Longrightarrow> set_array r x (set_array r' x' h) = set_array r' x' (set_array r x h)"
+  by (simp add: Let_def expand_fun_eq noteq_arrs_def set_array_def)
+
+lemma get_array_change_eq [simp]:
+  "get_array a (change a i v h) = (get_array a h) [i := v]"
+  by (simp add: change_def)
+
+lemma nth_change_array_neq_array [simp]:
+  "a =!!= b \<Longrightarrow> get_array a (change b j v h) ! i = get_array a h ! i"
+  by (simp add: change_def noteq_arrs_def)
+
+lemma get_arry_array_change_elem_neqIndex [simp]:
+  "i \<noteq> j \<Longrightarrow> get_array a (change a j v h) ! i = get_array a h ! i"
+  by simp
+
+lemma length_change [simp]: 
+  "length a (change b i v h) = length a h"
+  by (simp add: change_def length_def set_array_def get_array_def)
+
+lemma change_swap_neqArray:
+  "a =!!= a' \<Longrightarrow> 
+  change a i v (change a' i' v' h) 
+  = change a' i' v' (change a i v h)"
+apply (unfold change_def)
+apply simp
+apply (subst array_set_set_swap, assumption)
+apply (subst array_get_set_neq)
+apply (erule noteq_arrs_sym)
+apply (simp)
+done
+
+lemma change_swap_neqIndex:
+  "\<lbrakk> i \<noteq> i' \<rbrakk> \<Longrightarrow> change a i v (change a i' v' h) = change a i' v' (change a i v h)"
+  by (auto simp add: change_def array_set_set_swap list_update_swap)
+
+lemma get_array_init_array_list:
+  "get_array (fst (array ls h)) (snd (array ls' h)) = ls'"
+  by (simp add: Let_def split_def array_def)
+
+lemma set_array:
+  "set_array (fst (array ls h))
+     new_ls (snd (array ls h))
+       = snd (array new_ls h)"
+  by (simp add: Let_def split_def array_def)
+
+lemma array_present_change [simp]: 
+  "array_present a (change b i v h) = array_present a h"
+  by (simp add: change_def array_present_def set_array_def get_array_def)
+
+
+
 subsection {* Primitives *}
 
 definition
   new :: "nat \<Rightarrow> 'a\<Colon>heap \<Rightarrow> 'a array Heap" where
-  [code del]: "new n x = Heap_Monad.heap (Heap.array (replicate n x))"
+  [code del]: "new n x = Heap_Monad.heap (Array.array (replicate n x))"
 
 definition
   of_list :: "'a\<Colon>heap list \<Rightarrow> 'a array Heap" where
-  [code del]: "of_list xs = Heap_Monad.heap (Heap.array xs)"
+  [code del]: "of_list xs = Heap_Monad.heap (Array.array xs)"
 
 definition
-  length :: "'a\<Colon>heap array \<Rightarrow> nat Heap" where
-  [code del]: "length arr = Heap_Monad.heap (\<lambda>h. (Heap.length arr h, h))"
+  len :: "'a\<Colon>heap array \<Rightarrow> nat Heap" where
+  [code del]: "len arr = Heap_Monad.heap (\<lambda>h. (Array.length arr h, h))"
 
 definition
   nth :: "'a\<Colon>heap array \<Rightarrow> nat \<Rightarrow> 'a Heap"
 where
-  [code del]: "nth a i = (do len \<leftarrow> length a;
+  [code del]: "nth a i = (do len \<leftarrow> len a;
                  (if i < len
                      then Heap_Monad.heap (\<lambda>h. (get_array a h ! i, h))
                      else raise ''array lookup: index out of range'')
@@ -34,9 +142,9 @@ where
 definition
   upd :: "nat \<Rightarrow> 'a \<Rightarrow> 'a\<Colon>heap array \<Rightarrow> 'a\<Colon>heap array Heap"
 where
-  [code del]: "upd i x a = (do len \<leftarrow> length a;
+  [code del]: "upd i x a = (do len \<leftarrow> len a;
                       (if i < len
-                           then Heap_Monad.heap (\<lambda>h. (a, Heap.upd a i x h))
+                           then Heap_Monad.heap (\<lambda>h. (a, change a i x h))
                            else raise ''array update: index out of range'')
                    done)" 
 
@@ -73,7 +181,7 @@ definition
   freeze :: "'a\<Colon>heap array \<Rightarrow> 'a list Heap"
 where
   "freeze a = (do
-     n \<leftarrow> length a;
+     n \<leftarrow> len a;
      mapM (nth a) [0..<n]
    done)"
 
@@ -81,12 +189,11 @@ definition
    map :: "('a\<Colon>heap \<Rightarrow> 'a) \<Rightarrow> 'a array \<Rightarrow> 'a array Heap"
 where
   "map f a = (do
-     n \<leftarrow> length a;
+     n \<leftarrow> len a;
      mapM (\<lambda>n. map_entry n f a) [0..<n];
      return a
    done)"
 
-hide_const (open) new map -- {* avoid clashed with some popular names *}
 
 
 subsection {* Properties *}
@@ -125,12 +232,12 @@ lemma [code]:
   "Array.make n f = Array.make' (Code_Numeral.of_nat n) (f o Code_Numeral.nat_of)"
   by (simp add: make'_def o_def)
 
-definition length' where
-  [code del]: "length' a = Array.length a \<guillemotright>= (\<lambda>n. return (Code_Numeral.of_nat n))"
-hide_const (open) length'
+definition len' where
+  [code del]: "len' a = Array.len a \<guillemotright>= (\<lambda>n. return (Code_Numeral.of_nat n))"
+hide_const (open) len'
 lemma [code]:
-  "Array.length a = Array.length' a \<guillemotright>= (\<lambda>i. return (Code_Numeral.nat_of i))"
-  by (simp add: length'_def)
+  "Array.len a = Array.len' a \<guillemotright>= (\<lambda>i. return (Code_Numeral.nat_of i))"
+  by (simp add: len'_def)
 
 definition nth' where
   [code del]: "nth' a = Array.nth a o Code_Numeral.nat_of"
@@ -154,7 +261,7 @@ code_const Array (SML "raise/ (Fail/ \"bare Array\")")
 code_const Array.new' (SML "(fn/ ()/ =>/ Array.array/ ((_),/ (_)))")
 code_const Array.of_list' (SML "(fn/ ()/ =>/ Array.fromList/ _)")
 code_const Array.make' (SML "(fn/ ()/ =>/ Array.tabulate/ ((_),/ (_)))")
-code_const Array.length' (SML "(fn/ ()/ =>/ Array.length/ _)")
+code_const Array.len' (SML "(fn/ ()/ =>/ Array.length/ _)")
 code_const Array.nth' (SML "(fn/ ()/ =>/ Array.sub/ ((_),/ (_)))")
 code_const Array.upd' (SML "(fn/ ()/ =>/ Array.update/ ((_),/ (_),/ (_)))")
 
@@ -167,7 +274,7 @@ code_type array (OCaml "_/ array")
 code_const Array (OCaml "failwith/ \"bare Array\"")
 code_const Array.new' (OCaml "(fun/ ()/ ->/ Array.make/ (Big'_int.int'_of'_big'_int/ _)/ _)")
 code_const Array.of_list' (OCaml "(fun/ ()/ ->/ Array.of'_list/ _)")
-code_const Array.length' (OCaml "(fun/ ()/ ->/ Big'_int.big'_int'_of'_int/ (Array.length/ _))")
+code_const Array.len' (OCaml "(fun/ ()/ ->/ Big'_int.big'_int'_of'_int/ (Array.length/ _))")
 code_const Array.nth' (OCaml "(fun/ ()/ ->/ Array.get/ _/ (Big'_int.int'_of'_big'_int/ _))")
 code_const Array.upd' (OCaml "(fun/ ()/ ->/ Array.set/ _/ (Big'_int.int'_of'_big'_int/ _)/ _)")
 
@@ -180,8 +287,10 @@ code_type array (Haskell "Heap.STArray/ Heap.RealWorld/ _")
 code_const Array (Haskell "error/ \"bare Array\"")
 code_const Array.new' (Haskell "Heap.newArray/ (0,/ _)")
 code_const Array.of_list' (Haskell "Heap.newListArray/ (0,/ _)")
-code_const Array.length' (Haskell "Heap.lengthArray")
+code_const Array.len' (Haskell "Heap.lengthArray")
 code_const Array.nth' (Haskell "Heap.readArray")
 code_const Array.upd' (Haskell "Heap.writeArray")
+
+hide_const (open) new map -- {* avoid clashed with some popular names *}
 
 end
